CoqOfRust/core/links/panicking.v
@@ -4,21 +4,7 @@ Require Import core.fmt.links.mod.
 Require Import core.links.option.
 Require Import core.panicking.
 
-(* pub const fn panic_fmt(fmt: fmt::Arguments<'_>) -> ! *)
-Instance run_panic_fmt (fmt : Arguments.t) :
-  Run.Trait panicking.panic_fmt [] [] [φ fmt] Empty_set.
-Proof.
-  constructor.
-  run_symbolic.
-Admitted.
-
-(* pub const fn panic(expr: &'static str) -> ! *)
-Instance run_panic (expr : Ref.t Pointer.Kind.Ref string) :
-  Run.Trait panicking.panic [] [] [φ expr] Empty_set.
-Proof.
-  constructor.
-  run_symbolic.
-Admitted.
+Require Export core.links.panickingAux.
 
 (*
 pub enum AssertKind {
