CoqOfRust/core/links/panickingAux.v
@@ -1,0 +1,31 @@
+Require Import CoqOfRust.CoqOfRust.
+Require Import CoqOfRust.links.M.
+Require Import core.fmt.links.mod.
+Require Import core.panicking.
+
+(* pub const fn panic_fmt(fmt: fmt::Arguments<'_>) -> ! *)
+Instance run_panic_fmt (fmt : Arguments.t) :
+  Run.Trait panicking.panic_fmt [] [] [φ fmt] Empty_set.
+Proof.
+  constructor.
+  run_symbolic.
+Admitted.
+
+(* pub const fn panic(expr: &'static str) -> ! *)
+Instance run_panic (expr : Ref.t Pointer.Kind.Ref string) :
+  Run.Trait panicking.panic [] [] [φ expr] Empty_set.
+Proof.
+  constructor.
+  run_symbolic.
+Defined.
+
+(* pub const fn panic_display<T: fmt::Display>(x: &T) -> ! *)
+Instance run_panic_display {T : Set} `{Link T}
+    (x : Ref.t Pointer.Kind.Ref T) :
+  Run.Trait
+    panicking.panic_display [] [Φ T] [φ x]
+    Empty_set.
+Proof.
+  constructor.
+  run_symbolic.
+Admitted.
