CoqOfRust/revm/revm_interpreter/instructions/links/contract/extdelegatecall.v
@@ -65,4 +65,4 @@ Proof.
   destruct run_InputsTrait_for_Input.
   destruct run_RuntimeFlag_for_RuntimeFlag.
   run_symbolic.
-Defined.
+Admitted.
